\documentclass{article}

\usepackage{amsmath}

\begin{document}

\noindent {\bf Prior distribution for $\theta$:} \\

\[p(\theta) = p(\beta,\gamma)p(\nu)\]

\begin{align*}
R_0 &= \beta / \gamma \\
f(R_0,\gamma) &= p(R_0)p(\gamma) = \mbox{LN}(R_0;\mu_{R_0},\sigma^2_{R_0})\times\mbox{LN}(\gamma;\mu_{\gamma},\sigma^2_{\gamma})
\end{align*}

\begin{align*}
p(\beta,\gamma) &= f(\beta / \gamma, \gamma)\times|J| \\
|J| &= \left|\begin{array}{cc}
\frac{\mbox{d}R_0}{\mbox{d}\beta} & \frac{\mbox{d}R_0}{\mbox{d}\gamma} \\
\frac{\mbox{d}\gamma}{\mbox{d}\beta} & \frac{\mbox{d}\gamma}{\mbox{d}\gamma}
\end{array}
\right| = \left|\begin{array}{cc}
\frac{1}{\gamma} & -\frac{1}{\gamma^2} \\
0 & 1
\end{array}
\right| = 1 / \gamma
\end{align*}

\begin{align*}
p(\beta,\gamma) &= \frac{1}{\gamma}\times\mbox{LN}(\beta/\gamma;\mu_{R_0},\sigma^2_{R_0})\times\mbox{LN}(\gamma;\mu_{\gamma},\sigma^2_{\gamma}) \\
 &\propto \frac{1}{\gamma}\exp[-\frac{1}{2\sigma^2_{R_0}}(\log\frac{\beta}{\gamma} - \mu_{R_0})^2]\exp[-\frac{1}{2\sigma^2_{\gamma}}(\log\gamma - \mu_{\gamma})^2]
\end{align*}

\end{document}
